Revert to state of 8c28afb409c7 (add test file)

AesopTest/LazyForwardTest.lean
@@ -6,80 +6,24 @@ Authors: Xavier Généreux
 
 import Aesop
 
-section errors
-
-example {α β γ : Prop} (h : α → β → γ) (h₁ : α) (h₂ : β) (h : Empty) : False := by
-  set_option aesop.dev.statefulForward false in
-  --set_option trace.aesop true in
-  set_option trace.aesop true in
-  aesop (add safe forward h)
-
-end errors
+def myProp {i j : Type} (a : i) (b : j) : Prop := sorry
 
 variable {i j k l m n o p : Type}
 
--- def i : Type := sorry
--- def j : Type := sorry
--- def k : Type := sorry
--- def l : Type := sorry
--- def m : Type := sorry
--- def n : Type := sorry
--- def o : Type := sorry
--- def p : Type := sorry
-
-def myProp {I J : Type} (a : I) (b : J) : Prop := sorry
-
 theorem myThm (a : i) (b : j) (c : k) (d : l) :
-    myProp a b ↔ myProp c d := by
-  constructor
-  · intro hab
-    exact hab
-  sorry
+    myProp a b ↔ myProp c d := sorry
 
--- #check Aesop.BuiltinRules.empty_false
-
-example (h : Empty) : False := by
-  -- set_option aesop.dev.statefulForward true in
-  -- set_option trace.profiler.threshold 0 in
-  -- set_option trace.profiler true in
-  -- set_option trace.aesop true in
-  aesop
 
 example (a : i) (b : j) (c : k) (d : l) (e : m) (f : n) (g : o) (h : p) :
     myProp a b ↔ myProp c d := by
-  -- set_option aesop.dev.statefulForward true in
-  -- set_option trace.profiler.threshold 0 in
-  -- set_option trace.profiler true in
-  -- set_option trace.aesop.forward true in
-  aesop (add unsafe forward [myThm])
-
-example : True := by
-  -- set_option trace.aesop true in
-  aesop
-
-example (a : i) (b : j) (c : k) (d : l) (e : m) (f : n) (g : o) (h : p) :
-    True := by
-  -- set_option aesop.dev.statefulForward true in
-  -- set_option trace.profiler.threshold 0 in
-  -- set_option trace.profiler true in
-  -- set_option trace.aesop true in
-  aesop (add safe forward [myThm, True.intro])
-
-example (a : i) (b : j) (c : k) (d : l) (e : m) :
-    False := by
-  -- set_option aesop.dev.statefulForward true in
-  -- set_option trace.profiler.threshold 0 in
-  -- set_option trace.profiler true in
-  set_option trace.aesop.forward true in
-  try aesop (add unsafe forward [myThm])
-  sorry
-
-
-example (a b c d : Nat) (hab : a ≤ b) (hbc : b ≤ c) (hcd : c ≤ d) : a ≤ d := by
-  --set_option trace.profiler true in
-  set_option trace.aesop.forward true in
-  set_option aesop.dev.statefulForward true in
-  aesop (add unsafe forward Nat.le_trans)
+  set_option aesop.dev.statefulForward false in
+  set_option trace.profiler.threshold 0 in
+  set_option trace.profiler true in
+  --set_option trace.aesop true in
+  set_option maxHeartbeats 20000 in
+  -- saturate [myThm]
+  -- assumption
+  aesop (add safe forward myThm)
 
 /-
 This situation occurs in the case of `StdBasisMatrix.mul_same`. This is a deprecated lemma,
@@ -102,8 +46,5 @@ Thoughts:
 - It's kind of unfortunate that given `(a : i) (i : Type)` hypotheses like `inst✝ : Semiring α : Type` will get matched.
 - Overall this is a terrible forward rule - very general hypotheses + very specific thm. Maybe it would be interesting to run the benchmark where we add the rules both backwards and forwards and then interweave the process of both?
 - It is not clear to me why `oldForward` is faster, maybe it's running other stuff before trying to do forward reasoning? Indeed, if you run `saturate` than old is slower.
-
-I want to create the forward state associated to a rule only when we get for the first
-time to its phase.
 
 -/
