Aesop/Forward/State/Initial.lean
@@ -11,48 +11,32 @@ open Lean Lean.Meta
 
 namespace Aesop.LocalRuleSet
 
-def mkInitialForwardState (goal : MVarId) (forwardState : ForwardState) (rs : LocalRuleSet)
-    (phase : Option PhaseName) : BaseM (ForwardState × Array ForwardRuleMatch) :=
+def mkInitialForwardState (goal : MVarId) (rs : LocalRuleSet) :
+    BaseM (ForwardState × Array ForwardRuleMatch) :=
   goal.withContext do
-    aesop_trace![forward] "current forward state at begin init: {forwardState}"
     if ! aesop.dev.statefulForward.get (← getOptions) then
       -- We still initialise the hyp types since these are also used by
       -- stateless forward reasoning.
-      let mut hypTypes := forwardState.hypTypes
+      let mut hypTypes := ∅
       for ldecl in ← getLCtx do
         if ! ldecl.isImplementationDetail then
           hypTypes := hypTypes.insert (← rpinf ldecl.type)
-      -- IO.print "hypTypes: "
-      -- IO.println hypTypes.toList
-      return ({ forwardState with hypTypes }, #[])
-    let mut fs : ForwardState := forwardState
-    let mut ruleMatches := rs.constForwardRuleMatches.filter (·.rule.name.phase == phase)
+      return ({ (∅ : ForwardState) with hypTypes }, #[])
+    let mut fs : ForwardState := ∅
+    let mut ruleMatches := rs.constForwardRuleMatches
     aesop_trace[forward] do
       for m in ruleMatches do
         aesop_trace![forward] "match for constant rule {m.rule.name}"
     for ldecl in ← show MetaM _ from getLCtx do
       if ldecl.isImplementationDetail then
         continue
-      let mut rules := default
-      -- Would it be more efficient to do one filter outside the loop?
-      match phase with
-      | some phase =>
-        rules ← rs.applicableForwardRulesWith ldecl.type (·.name.phase == phase)
-      | none => rules ← rs.applicableForwardRules ldecl.type
-      let patInsts := ← rs.forwardRulePatternSubstsInLocalDecl ldecl
+      let rules ← rs.applicableForwardRules ldecl.type
+      let patInsts ← rs.forwardRulePatternSubstsInLocalDecl ldecl
       let (fs', ruleMatches') ←
         fs.addHypWithPatSubstsCore ruleMatches goal ldecl.fvarId rules patInsts
-      fs := {fs' with phaseProgress := phase}
+      fs := fs'
       ruleMatches := ruleMatches'
-    -- IO.println "constructing forward state for phase: "
-    -- IO.print phase
-    -- IO.print "with rules: "
-    -- IO.println (fs.ruleStates.toList.map (·.1))
-    -- IO.println (ruleMatches.map (·.rule))
     let patInsts ← rs.forwardRulePatternSubstsInExpr (← goal.getType)
-    let rs ← fs.addPatSubstsCore ruleMatches goal patInsts
-    -- IO.println (rs.1.ruleStates.toList.map (·.1))
-    -- IO.println (rs.2.map (·.rule))
-    return rs
+    fs.addPatSubstsCore ruleMatches goal patInsts
 
 end Aesop.LocalRuleSet
